Weidenbach_Book/Watched_Literals_All_Literals.thy
@@ -1,5 +1,5 @@
 theory Watched_Literals_All_Literals
-imports Watched_Literals_List
+imports Watched_Literals_Clauses
 begin
 
 type_synonym ann_lits_l = \<open>(nat, nat) ann_lits\<close>
@@ -9,6 +9,71 @@ type_synonym clauses_to_update_ll = \<open>nat list\<close>
 subsection \<open>Refinement\<close>
 
 subsubsection \<open>Set of all literals of the problem\<close>
+
+
+definition all_lits_of_mm :: \<open>'a clauses \<Rightarrow> 'a literal multiset\<close> where
+\<open>all_lits_of_mm Ls = Pos `# (atm_of `# (\<Union># Ls)) + Neg `# (atm_of `# (\<Union># Ls))\<close>
+
+lemma all_lits_of_mm_empty[simp]: \<open>all_lits_of_mm {#} = {#}\<close>
+  by (auto simp: all_lits_of_mm_def)
+lemma in_all_lits_of_mm_ain_atms_of_iff:
+  \<open>L \<in># all_lits_of_mm N \<longleftrightarrow> atm_of L \<in> atms_of_mm N\<close>
+  by (cases L) (auto simp: all_lits_of_mm_def atms_of_ms_def atms_of_def)
+
+lemma all_lits_of_mm_union:
+  \<open>all_lits_of_mm (M + N) = all_lits_of_mm M + all_lits_of_mm N\<close>
+  unfolding all_lits_of_mm_def by auto
+
+definition all_lits_of_m :: \<open>'a clause \<Rightarrow> 'a literal multiset\<close> where
+  \<open>all_lits_of_m Ls = Pos `# (atm_of `# Ls) + Neg `# (atm_of `# Ls)\<close>
+
+lemma all_lits_of_m_empty[simp]: \<open>all_lits_of_m {#} = {#}\<close>
+  by (auto simp: all_lits_of_m_def)
+
+lemma all_lits_of_m_empty_iff[iff]: \<open>all_lits_of_m A = {#} \<longleftrightarrow> A = {#}\<close>
+  by (cases A) (auto simp: all_lits_of_m_def)
+
+lemma in_all_lits_of_m_ain_atms_of_iff: \<open>L \<in># all_lits_of_m N \<longleftrightarrow> atm_of L \<in> atms_of N\<close>
+  by (cases L) (auto simp: all_lits_of_m_def atms_of_ms_def atms_of_def)
+
+lemma in_clause_in_all_lits_of_m: \<open>x \<in># C \<Longrightarrow> x \<in># all_lits_of_m C\<close>
+  using atm_of_lit_in_atms_of in_all_lits_of_m_ain_atms_of_iff by blast
+
+lemma all_lits_of_mm_add_mset:
+  \<open>all_lits_of_mm (add_mset C N) = (all_lits_of_m C) + (all_lits_of_mm N)\<close>
+  by (auto simp: all_lits_of_mm_def all_lits_of_m_def)
+
+lemma all_lits_of_m_add_mset:
+  \<open>all_lits_of_m (add_mset L C) = add_mset L (add_mset (-L) (all_lits_of_m C))\<close>
+  by (cases L) (auto simp: all_lits_of_m_def)
+
+lemma all_lits_of_m_union:
+  \<open>all_lits_of_m (A + B) = all_lits_of_m A + all_lits_of_m B\<close>
+  by (auto simp: all_lits_of_m_def)
+
+lemma all_lits_of_m_mono:
+  \<open>D \<subseteq># D' \<Longrightarrow> all_lits_of_m D \<subseteq># all_lits_of_m D'\<close>
+  by (auto elim!: mset_le_addE simp: all_lits_of_m_union)
+
+lemma in_all_lits_of_mm_uminusD: \<open>x2 \<in># all_lits_of_mm N \<Longrightarrow> -x2 \<in># all_lits_of_mm N\<close>
+  by (auto simp: all_lits_of_mm_def)
+
+lemma in_all_lits_of_mm_uminus_iff: \<open>-x2 \<in># all_lits_of_mm N \<longleftrightarrow> x2 \<in># all_lits_of_mm N\<close>
+  by (cases x2) (auto simp: all_lits_of_mm_def)
+
+lemma all_lits_of_mm_diffD:
+  \<open>L \<in># all_lits_of_mm (A - B) \<Longrightarrow> L \<in># all_lits_of_mm A\<close>
+  apply (induction A arbitrary: B)
+  subgoal by auto
+  subgoal for a A' B
+    by (cases \<open>a \<in># B\<close>)
+      (fastforce dest!: multi_member_split[of a B] simp: all_lits_of_mm_add_mset)+
+  done
+
+lemma all_lits_of_mm_mono:
+  \<open>set_mset A \<subseteq> set_mset B \<Longrightarrow> set_mset (all_lits_of_mm A) \<subseteq> set_mset (all_lits_of_mm B)\<close>
+  by (auto simp: all_lits_of_mm_def)
+
 
 text \<open>We start in a context where we have an initial set of atoms. We later extend the locale to
   include a bound on the largest atom (in order to generate more efficient code).
